src/Std/Data/ExtHashSet/Basic.lean
@@ -205,6 +205,16 @@ def union [EquivBEq α] [LawfulHashable α] (m₁ m₂ : ExtHashSet α) : ExtHas
 instance [EquivBEq α] [LawfulHashable α] : Union (ExtHashSet α) := ⟨union⟩
 
 /--
+Computes the intersection of the given hash sets.
+
+This function always iterates through the smaller set.
+-/
+@[inline]
+def inter [EquivBEq α] [LawfulHashable α] (m₁ m₂ : ExtHashSet α) : ExtHashSet α := ⟨ExtHashMap.inter m₁.inner m₂.inner⟩
+
+instance [EquivBEq α] [LawfulHashable α] : Inter (ExtHashSet α) := ⟨inter⟩
+
+/--
 Creates a hash set from an array of elements. Note that unlike repeatedly calling `insert`, if the
 collection contains multiple elements that are equal (with regard to `==`), then the last element
 in the collection will be present in the returned hash set.
