src/Std/Data/DHashMap/Raw.lean
@@ -766,11 +766,13 @@ theorem WF.union₀ [BEq α] [Hashable α] {m₁ m₂ : Raw α β} (h₁ : m₁.
   . exact (Raw₀.insertManyIfNew ⟨m₂, h₂.size_buckets_pos⟩ m₁).2 _ WF.insertIfNew₀ h₂
   . exact (Raw₀.insertMany ⟨m₁, h₁.size_buckets_pos⟩ m₂).2 _ WF.insert₀ h₁
 
-theorem WF.union [BEq α] [Hashable α] {m₁ m₂ : Raw α β} (h₁ : m₁.WF) (h₂ : m₂.WF) : (m₁.union m₂ : Raw α β).WF := by
+theorem WF.union [BEq α] [Hashable α] {m₁ m₂ : Raw α β} (h₁ : m₁.WF) (h₂ : m₂.WF) : (m₁ ∪ m₂ : Raw α β).WF := by
+  simp only [Union.union]
   simp [Std.DHashMap.Raw.union, h₁.size_buckets_pos, h₂.size_buckets_pos]
   exact WF.union₀ h₁ h₂
 
-theorem WF.inter [BEq α] [Hashable α] {m₁ m₂ : Raw α β} (h₁ : m₁.WF) (h₂ : m₂.WF) : (m₁.inter m₂ : Raw α β).WF := by
+theorem WF.inter [BEq α] [Hashable α] {m₁ m₂ : Raw α β} (h₁ : m₁.WF) (h₂ : m₂.WF) : (m₁ ∩ m₂ : Raw α β).WF := by
+  simp only [Inter.inter]
   simp [Std.DHashMap.Raw.inter, h₁.size_buckets_pos, h₂.size_buckets_pos]
   exact WF.inter₀ h₁ h₂
 
