src/Std/Data/HashMap/RawLemmas.lean
@@ -1568,6 +1568,22 @@ theorem not_mem_inter_of_not_mem_right [EquivBEq α] [LawfulHashable α]
     k ∉ m₁ ∩ m₂ :=
   @DHashMap.Raw.not_mem_inter_of_not_mem_right _ _ _ _ m₁.inner m₂.inner _ _ h₁.out h₂.out k not_mem
 
+/- Equiv -/
+theorem Equiv.inter_left {m₃ : Raw α β} [EquivBEq α] [LawfulHashable α] (h₁ : m₁.WF) (h₂ : m₂.WF) (h₃ : m₃.WF)
+    (equiv : m₁ ~m m₂) :
+    (m₁ ∩ m₃) ~m (m₂ ∩ m₃) :=
+  ⟨@DHashMap.Raw.Equiv.inter_left _ _ _ _ m₁.inner m₂.inner m₃.inner _ _ h₁.out h₂.out h₃.out equiv.1⟩
+
+theorem Equiv.inter_right {m₃ : Raw α β} [EquivBEq α] [LawfulHashable α] (h₁ : m₁.WF) (h₂ : m₂.WF) (h₃ : m₃.WF)
+    (equiv : m₂ ~m m₃) :
+    (m₁ ∩ m₂) ~m (m₁ ∩ m₃) :=
+  ⟨@DHashMap.Raw.Equiv.inter_right _ _ _ _ m₁.inner m₂.inner m₃.inner _ _ h₁.out h₂.out h₃.out equiv.1⟩
+
+theorem Equiv.inter_congr {m₃ m₄ : Raw α β} [EquivBEq α] [LawfulHashable α] (h₁ : m₁.WF) (h₂ : m₂.WF) (h₃ : m₃.WF) (h₄ : m₄.WF)
+    (equiv₁ : m₁ ~m m₃) (equiv₂ : m₂ ~m m₄) :
+    (m₁ ∩ m₂) ~m (m₃ ∩ m₄) :=
+  ⟨@DHashMap.Raw.Equiv.inter_congr _ _ _ _ m₁.inner m₂.inner m₃.inner m₄.inner _ _ h₁.out h₂.out h₃.out h₄.out equiv₁.1 equiv₂.1⟩
+
 /- get? -/
 theorem get?_inter [EquivBEq α] [LawfulHashable α] (h₁ : m₁.WF) (h₂ : m₂.WF) {k : α} :
     get? (m₁ ∩ m₂) k =
